Joinable.v
@@ -1,0 +1,111 @@
+Require Import AbstractStore.
+Require Import Parity.
+Require Import Preorder.
+
+Class Joinable (T : Type) `{PreorderedSet T} : Type :=
+{
+  join_op : T -> T -> T;
+  join_upper_bound: forall t t', preorder t (join_op t t');
+  join_comm : forall t t', join_op t t' = join_op t' t;
+}.
+
+Lemma parity_join_upperbound :
+  forall p p', preorder p (parity_join p p').
+Proof.
+  intros. simpl. unfold parity_join. destruct p, p'; constructor.
+Qed.
+
+Instance parity_joinable : Joinable parity := {
+  join_op := parity_join;
+  join_upper_bound := parity_join_upperbound;
+  join_comm := parity_join_comm;
+}.
+
+Section option_joinable.
+Context {A} `{Joinable A}.
+Definition option_join (o1 o2 : option A) : option A :=
+  match o1, o2 with
+  | Some x, Some y => Some (join_op x y)
+  | _, _ => None
+  end.
+
+Lemma option_join_upperbound : forall o o', preorder o (option_join o o').
+Proof.
+  intros. simpl. destruct o, o'; constructor.
+  apply join_upper_bound.
+Qed.
+
+Lemma option_join_comm : forall o o', option_join o o' = option_join o' o.
+Proof.
+  intros. destruct o, o'; try reflexivity.
+  unfold option_join. rewrite join_comm. reflexivity.
+Qed.
+
+Global Instance option_joinable : Joinable (option A) := 
+{
+  join_op := option_join;
+  join_upper_bound := option_join_upperbound;
+  join_comm := option_join_comm;
+}.
+
+End option_joinable.
+
+Section pair_joinable.
+Context {A B} `{Joinable A, Joinable B}.
+
+Definition pair_join (p1 p2 : A*B) : A*B :=
+  ((join_op (fst p1) (fst p2)), (join_op (snd p1) (snd p2))).
+
+Lemma pair_join_upperbound : forall p p', 
+  preorder p (pair_join p p').
+Proof.
+  intros. simpl. destruct p, p'. constructor;
+  simpl; apply join_upper_bound.
+Qed.
+
+Lemma pair_join_comm : forall p p',
+  pair_join p p' = pair_join p' p.
+Proof.
+  unfold pair_join. intros. rewrite -> join_comm. 
+  replace (join_op (snd p )(snd p')) with (join_op (snd p') (snd p)).
+  reflexivity. apply join_comm.
+Qed.
+
+Global Instance pair_joinable : Joinable (prod A B) :=
+{
+  join_op := pair_join;
+  join_upper_bound := pair_join_upperbound;
+  join_comm := pair_join_comm;
+}.
+End pair_joinable.
+
+Instance abstract_store_joinable : Joinable abstract_store := {
+  join_op := abstract_store_join;
+  join_comm := abstract_store_join_comm;
+}.
+Proof.
+simpl. unfold abstract_store_join. constructor.  
+intro x. apply parity_join_upperbound.
+Defined.
+
+Section unit_joinable.
+
+Definition unit_join : unit -> unit -> unit :=
+  fun _ _ => tt.
+
+Lemma unit_join_upperbound : forall (u u' : unit),
+  preorder u (unit_join u u').
+Proof.
+  intros. destruct u, u'. unfold unit_join. apply preorder_refl.
+Qed.
+
+Global Instance unit_joinable : Joinable unit :=
+{
+  join_op := unit_join;
+  join_upper_bound := unit_join_upperbound;
+}.
+Proof.
+  destruct t, t'. reflexivity.
+Defined.
+End unit_joinable.
+
